two counters with same type but different local state, proving small property that two applications of these are observationally equivalent

examples/dm4free/Relational.ProgramEquivalence.fst
@@ -1,6 +1,6 @@
 module Relational.ProgramEquivalence
 
-open FStar.Set
+open FStar.List.Tot
 open FStar.DM4F.Heap
 open FStar.DM4F.Heap.ST
 
@@ -29,29 +29,68 @@ open FStar.DM4F.Heap.ST
 (* 	                         (sel h_1 r == sel h_0 r /\ *)
 (* 				  sel h_2 r == sel h_0 r))) *)
 
-(* let contains_a_well_typed_set (h:heap) (s:set nat) = *)
-(*   forall (a:Type) (r:ref a). mem (addr_of r) s ==> h `contains_a_well_typed` r *)
+let contains_well_typed_refs (h:heap) (s:list (ref nat)) =
+  forall (r:ref nat). memP r s ==> h `contains_a_well_typed` r
 
-(* noeq type t = *)
-(*   | C: s:set nat -> (unit -> ST nat (requires (fun h0      -> h0 `contains_a_well_typed_set` s)) *)
-(*                                (ensures  (fun h0 _ h1 -> h1 `contains_a_well_typed_set` s))) *)
-(*        -> t		     *)
+type fp = l:list (ref nat)
 
-(* reifiable let ctr_0 () :STNull t = *)
-(*   let r = alloc_weak 0 in *)
-(*   let f = fun () -> read_weak r in *)
-(*   C (singleton (addr_of r)) f *)
+type ctr (inv:heap -> fp -> Type0) =
+  s:fp
+  -> ST nat (requires (fun h0       -> inv h0 s))
+          (ensures  (fun h0 _ h1 -> inv h1 s))
 
-(* let ctr0_obs (h_0:heap) :unit = *)
-(*   let x, h_1 = reify (ctr_0 ()) h_0 in *)
-(*   match x with *)
-(*   | C _ f -> *)
-(*     let r, h_2 = reify (f ()) h_1 in *)
-(*     assert (r = 0) *)
+noeq abstract type t =
+  | C: inv:(heap -> fp -> Type0) -> fp:fp -> c:(ctr inv) -> t
 
-reifiable let foo (r:ref nat) :ST nat (requires (fun h0 -> h0 `contains_a_well_typed` r)) (ensures (fun _ _ _ -> True)) =
-  let g = !r in
-  let f = fun () -> !r in
-  f ()
+abstract let good_t (t:t) (h:heap) = (C?.inv t) h (C?.fp t)
 
-let foo_obs (r:ref nat) (h0:heap) :nat = 2
+abstract let inv_0 (h:heap) (fp:fp) :Type0 =
+  h `contains_well_typed_refs` fp /\
+  length fp = 1
+
+reifiable private let incr_0 :(ctr inv_0) =
+  fun s ->
+    let r = hd s in
+    let c = read_weak r in
+    write_weak r (c + 2);
+    c
+
+reifiable let ctr_0 () :ST t (requires (fun h0 -> True)) (ensures (fun _ r h1 -> good_t r h1))
+  = let r = alloc_weak 2 in
+    C inv_0 [r] incr_0
+
+abstract let inv_1 (h:heap) (fp:fp) :Type0 =
+  h `contains_well_typed_refs` fp /\
+  length fp = 2
+
+reifiable private let incr_1 :(ctr inv_1) =
+  fun s ->
+    let r_1 = hd s in
+    let r_2 = hd (tl s) in
+    let c_1 = read_weak r_1 in
+    let c_2 = read_weak r_2 in
+    write_weak r_1 (c_1 + 1);
+    write_weak r_2 (c_2 + 1);
+    c_1 + c_2
+
+reifiable let ctr_1 (): ST t (requires (fun h0 -> True)) (ensures (fun _ r h1 -> good_t r h1))
+  = let r_1 = alloc_weak 1 in
+    let r_2 = alloc_weak 1 in
+    C inv_1 [r_1; r_2] incr_1
+
+
+let ctr0_ctr1_obs (h:heap) :unit =
+  let c0, h0 = reify (ctr_0 ()) h in
+  let c1, h1 = reify (ctr_1 ()) h in
+
+  let n, h0 =
+    match c0 with
+    | C _ s f -> reify (let _ = f s in f s) h0
+  in
+  let m, h1 =
+    match c1 with
+    | C _ s f -> reify (let _ = f s in f s) h1
+  in
+  assert (n = m /\
+          (forall (a:Type) (r:ref a). h `contains` r ==> (sel h r == sel h0 r /\
+	                                             sel h r == sel h1 r)))
